Source clean up and formatting, prepare for print

src/semantics.lean
@@ -4,150 +4,113 @@ import syntax data.stream
 
 open stream signature type pexp nat
 
-/-
-We have the following class of dynamic types.
-Given a finite set,
-there can always be given a fresh instance not in that set.
-(with thanks to Johannes Hölzl)
--/
+/- We have the following class of dynamic types. Given a finite set, there can always be given a fresh instance not in that set. (Thanks to Johannes Hölzl!) -/
 class dynamic (β : Type) :=
 (fresh: finset β → β)
 (fresh_is_new: ∀x : finset β, (fresh x) ∉ x)
 open dynamic
 
-/-
-Fix a signature (and global names).
-We treat objects transparently.
-Each object is associated to a single class name.
-Equality is decidable for objects of the same class.
-Given a set of objects, we can always construct some new object.
--/
+/- Fix a signature (and global names). We treat objects transparently. Each object is associated to a single class name. Equality is decidable for objects of the same class. Given a set of objects, we can always construct some new object. -/
 class objects (α β : Type) extends signature α, dynamic β :=
 (class_of: β → class_name α)
 (equality (x y : β): class_of x = class_of y → bool)
 open objects
 
-/-
-We treat values as being of a type.
-A value of a reference type is an object of the same class.
-A value of a data type is a term of the type in the host language.
--/
-inductive value {α : Type} (β : Type) [objects α β] : type α → Type 1
+/- We treat values as being of a type. A value of a reference type is an object of the same class. A value of a data type is a term of the type in the host language. -/
+inductive value {α : Type} (β : Type) [objects α β] :
+  type α → Type 1
 | object (o : β) : value (ref (class_of α o))
 | term {γ : Type} : γ → value (data α γ)
 
 -- Projection of value to object
-def value.objective {α β : Type} [objects α β] {c : class_name α}
-(x : value β (ref c)) : β :=
+def value.objective {α β : Type} [objects α β]
+  {c : class_name α} (x : value β (ref c)) : β :=
 begin cases x, apply x_1 end
 
-lemma value.obj_class {α β : Type} [objects α β] {c : class_name α}
-(x : value β (ref c)) : class_of α (value.objective x) = c :=
+lemma value.obj_class {α β : Type} [objects α β]
+  {c : class_name α} (x : value β (ref c)) :
+  class_of α (value.objective x) = c :=
 begin cases x, unfold value.objective end
 
 -- Projection of value to term
-def value.terminal {α : Type} (β : Type) [objects α β] {γ : Type}
-(x : value β (data α γ)) : γ :=
+def value.terminal {α : Type} (β : Type) [objects α β]
+  {γ : Type} (x : value β (data α γ)) : γ :=
 begin cases x, apply x_a end
 
-/-
-Given two values of reference type,
-we can decide referential equality.
--/
-def value.ref_equal {α β : Type} [objects α β] {c : class_name α}
-(x : value β (ref c)) (y : value β (ref c)) : bool :=
+/- Given two values of reference type, we can decide referential equality. -/
+def value.ref_equal {α β : Type} [objects α β]
+  {c : class_name α} (x : value β (ref c))
+  (y : value β (ref c)) : bool :=
 let H : class_of α (value.objective x) =
-    class_of α (value.objective y) := begin
-    repeat {rewrite value.obj_class}
-end in equality (value.objective x) (value.objective y) H
+    class_of α (value.objective y) :=
+  begin repeat {rewrite value.obj_class} end
+in equality (value.objective x) (value.objective y) H
 
 open value
 
-/-
-For class C we have a state space Σ(C) consisting of:
-an assignment of fields to values.
--/
+/- For class C we have a state space Σ(C) consisting of: an assignment of fields to values. -/
 structure state_space {α : Type} (β : Type) [objects α β]
-(self : class_name α) : Type 1 :=
+  (self : class_name α) : Type 1 :=
 (map (f : field_name self) : value β (field_type f))
 
-/-
-Given a list of types,
-we have a value list of values with matching types.
--/
-inductive vallist {α : Type} (β : Type) [objects α β] : list (type α) → Type 1
+/- Given a list of types, we have a value list of values with matching types. -/
+inductive vallist {α : Type} (β : Type) [objects α β] :
+  list (type α) → Type 1
 | nil : vallist []
 | cons {x : type α} {xs : list (type α)} :
-    value β x → vallist xs → vallist (x::xs)
+  value β x → vallist xs → vallist (x::xs)
 
-/-
-Given a value list, and an index of its type list, we can obtain a value.
--/
+/- Given a value list, and an index of its type list, we can obtain a value. -/
 def vallist.lookup {α β : Type} [objects α β] :
-Π {l : context α} {ty : type α}, vallist β l → list_at ty l → value β ty
+  Π {l : context α} {ty : type α}, vallist β l → list_at ty l →
+  value β ty
 | (x :: xs) ._ (vallist.cons (v : value β x) _)
-    (list_at.head .(x) .(xs)) := v
+  (list_at.head .(x) .(xs)) := v
 | (x :: xs) ty (vallist.cons _ (ys : vallist β xs))
-    (list_at.tail .(x) (zs : list_at .(ty) xs)) := vallist.lookup ys zs
+  (list_at.tail .(x) (zs : list_at .(ty) xs)) :=
+    vallist.lookup ys zs
 
-/-
-Given a signature and method name m,
-we have a argument space Σ(m) consisting
-an assignment of method parameters to values.
--/
+/- Given a signature and method name m, we have a argument space Σ(m) consisting an assignment of method parameters to values. -/
 structure arg_space {α : Type} (β : Type) [objects α β]
-{self : class_name α} (m : method_name self) : Type 1 :=
+  {self : class_name α} (m : method_name self) : Type 1 :=
 (map : vallist β (method_params m))
 
-/-
-Given a type environment,
-we consider an assignment to consist of:
-a state space (of the self class),
-an argument space (of the current method),
-a value list (of the local variables)
--/
-structure assignment {α : Type} (β : Type) [objects α β] (e : tenv α) :=
+/- Given a type environment, we consider an assignment to consist of: a state space (of the self class), an argument space (of the current method), a value list (of the local variables) -/
+structure assignment {α : Type} (β : Type) [objects α β]
+  (e : tenv α) :=
 (state : state_space β e.self)
 (args : arg_space β e.current)
 (store : vallist β e.locals)
 
 def assignment.lookup {α β : Type} [objects α β] {e : tenv α}
-(σ : assignment β e) (tx : type α) : rvar e tx → value β tx
+  (σ : assignment β e) (tx : type α) : rvar e tx → value β tx
 | (rvar.fvar f) := eq.mpr (congr_arg _ f.H) (σ.state.map f.idx)
 | (rvar.pvar p) := σ.args.map.lookup p.idx
 | (rvar.lvar l) := σ.store.lookup l.idx
 
-/-
-NOTE: the definition for (rvar.fvar f) was found by the following proof,
+/- NOTE: the definition for (rvar.fvar f) was found by the following proof,
 for matching the type of tx to that of the field.
 
 begin
     have H : (tx = field_type f.idx), apply f.H,
     rewrite H,
     exact σ.state.map f.idx
-end
--/
+end -/
 
-/-
-Evaluating a pure expression in an assignment.
--/
-def peval {α β : Type} [objects α β] {e : tenv α} (σ : assignment β e)
-: Π {ty : type α}, pexp e ty → value β ty
+/- Evaluating a pure expression in an assignment. -/
+def peval {α β : Type} [objects α β] {e : tenv α}
+  (σ : assignment β e) : Π {ty : type α}, pexp e ty → value β ty
 | bool (requal (c : class_name α)
-  (l : pexp e (ref c)) (r : pexp e (ref c))) :=
-    term β (ref_equal (peval l) (peval r))
+    (l : pexp e (ref c)) (r : pexp e (ref c))) :=
+  term β (ref_equal (peval l) (peval r))
 | ty (lookup (r : rvar e ty)) := σ.lookup ty r
 | _ (value _ (γ : Type) (v : γ)) := term β v
-| _ (apply (γ : Type) δ
-  (pl : pexp e (γ → δ))
-  (pr : pexp e γ)) :=
-    term β ((terminal β (peval pl)) (terminal β (peval pr)))
+| _ (apply (γ : Type) δ (pl : pexp e (γ → δ)) (pr : pexp e γ)) :=
+  term β ((terminal β (peval pl)) (terminal β (peval pr)))
 
-/-
-Evaluating a statement in an assignment
-generates a stream of assignments.
--/
-def eval {α β : Type} [objects α β] {e : tenv α} (σ : assignment β e)
-: stmt e → stream (option (assignment β e))
+/- Evaluating a statement in an assignment generates a stream of assignments. -/
+def eval {α β : Type} [objects α β] {e : tenv α}
+  (σ : assignment β e) : stmt e →
+  stream (option (assignment β e))
 | (stmt.skip e) := cons σ (const none)
-| (stmt.seq l r) := sorry
+| _ := sorry
